Lean4Lean/Tests.lean
@@ -1,5 +1,6 @@
 import Lean4Lean.Tests.Toolchain
 import Lean4Lean.Tests.Environment
+import Lean4Lean.Tests.UniformIndOccs
 import Lean4Lean.Tests.LevelStd
 import Lean4Lean.Tests.LiteralReadiness
 import Lean4Lean.Tests.NotationPreludeReplay
